src/bva/Bva_checker.v
@@ -14,7 +14,6 @@
 
 (** A small checker for bit-vectors bit-blasting *)
 
-Add Rec LoadPath "." as SMTCoq.
 Require Import Int63 Int63Properties PArray.
 
 Require Import Misc State SMT_terms BVList Psatz.
@@ -2413,7 +2412,7 @@ Proof.
       case_eq (t_form .[ Lit.blit lres]); try (intros; now apply C.interp_true).
       intros a bsres Heq8.
       case_eq (t_atom .[ a]); try (intros; now apply C.interp_true).
-      intros [ | | | | | | | [ A B | A | | | | ]|N|N|N|N|N|N|N|N|N] a1' a2' Heq9; try now apply C.interp_true.
+      intros [ | | | | | | | [ A B | A | | | | ]|N|N|N|N|N|N|N|N| | ] a1' a2' Heq9; try now apply C.interp_true.
       (* BVand *)
       - case_eq ((a1 == a1') && (a2 == a2') || (a1 == a2') && (a2 == a1')); simpl; intros Heq10; try (now apply C.interp_true).
 
@@ -3465,7 +3464,7 @@ Lemma valid_check_bbEq pos1 pos2 lres : C.valid rho (check_bbEq pos1 pos2 lres).
        case_eq (t_form .[ Lit.blit a]); try (intros; now apply C.interp_true). intros a3 Heq10.
        case_eq (t_atom .[ a3]); try (intros; now apply C.interp_true).
 
-      intros [ | | | | | | | [ A B | A | | | | ]|N|N|N|N|N|N|N|N|N] a1' a2' Heq9; try now apply C.interp_true.
+      intros [ | | | | | | | [ A B | A | | | | ]|N|N|N|N|N|N|N|N| | ] a1' a2' Heq9; try now apply C.interp_true.
 
        case_eq ((a1 == a1') && (a2 == a2') || (a1 == a2') && (a2 == a1')); simpl; intros Heq15; try (now apply C.interp_true).
        
@@ -4069,7 +4068,7 @@ Proof.
        case_eq (t_form .[ Lit.blit a]); try (intros; now apply C.interp_true). intros a3 Heq10.
        case_eq (t_atom .[ a3]); try (intros; now apply C.interp_true).
 
-      intros [ | | | | | | | [ A B | A | | | | ]|N|N|N|N|N|N|N|N|N] a1' a2' Heq9; try now apply C.interp_true.
+      intros [ | | | | | | | [ A B | A | | | | ]|N|N|N|N|N|N|N|N| | ] a1' a2' Heq9; try now apply C.interp_true.
 
        case_eq ((a1 == a1') && (a2 == a2')); simpl; intros Heq15; try (now apply C.interp_true).
        
@@ -4271,7 +4270,7 @@ Proof.
        case_eq (t_form .[ Lit.blit a]); try (intros; now apply C.interp_true). intros a3 Heq10.
        case_eq (t_atom .[ a3]); try (intros; now apply C.interp_true).
 
-      intros [ | | | | | | | [ A B | A | | | | ]|N|N|N|N|N|N|N|N|N] a1' a2' Heq9; try now apply C.interp_true.
+      intros [ | | | | | | | [ A B | A | | | | ]|N|N|N|N|N|N|N|N| | ] a1' a2' Heq9; try now apply C.interp_true.
 
        case_eq ((a1 == a1') && (a2 == a2')); simpl; intros Heq15; try (now apply C.interp_true).
        
@@ -4690,7 +4689,7 @@ Proof.
       case_eq (t_form .[ Lit.blit lres]); try (intros; now apply C.interp_true).
       intros a bsres Heq8.
       case_eq (t_atom .[ a]); try (intros; now apply C.interp_true).
-      intros [ | | | | | | |[ A B | A| | | | ]|N|N|N|N|N|N|N|N|N] a1' a2' Heq9; try now apply C.interp_true.
+      intros [ | | | | | | |[ A B | A| | | | ]|N|N|N|N|N|N|N|N| | ] a1' a2' Heq9; try now apply C.interp_true.
       (* BVadd *)
       - case_eq ((a1 == a1') && (a2 == a2') || (a1 == a2') && (a2 == a1')); simpl; intros Heq10; try (now apply C.interp_true).
         case_eq (
@@ -5370,7 +5369,7 @@ Proof.
       case_eq (t_form .[ Lit.blit lres]); try (intros; now apply C.interp_true).
       intros a bsres Heq8.
       case_eq (t_atom .[ a]); try (intros; now apply C.interp_true).
-      intros [ | | | | | | |[ A B | A| | | | ]|N|N|N|N|N|N|N|N|N] a1' a2' Heq9; try now apply C.interp_true.
+      intros [ | | | | | | |[ A B | A| | | | ]|N|N|N|N|N|N|N|N| | ] a1' a2' Heq9; try now apply C.interp_true.
       (* BVmult *)
       - case_eq ((a1 == a1') && (a2 == a2') (* || (a1 == a2') && (a2 == a1')*) ); simpl; intros Heq10; try (now apply C.interp_true).
       
